WIP paper delta

lambda2Gmu/Equations.v
@@ -4,88 +4,182 @@ Require Import TLC.LibTactics.
 Require Import List.
 Import List.ListNotations.
 
+(*
+This file is a work in progress.
+It tries to prove that the original definition of semantic entailment of type equalities is equivalent with a simpler definition where order of equations and variables does not matter.
+The latter might be easier for usage in proofs, but I decided to pause proving this equivalence until I really actually need it.
+*)
+
 Section TypCtxDefEquivalence.
   (* Here we present the typctx defined precisely as in the paper and show that these two notions are essentially equivalent *)
 
-Inductive typctx_elem : Set :=
-| tc_var (A : var)
-| tc_eq (eq : type_equation).
+Record typctx' : Type := mkΔ {
+                           Δvars : fset var;
+                           Δeqs : fset type_equation
+                         }.
 
-(* we keep the elements in reverse order, i.e. the head is the last added element *)
-Definition typctx' := list typctx_elem.
+Definition add_var' (Δ : typctx') (A : var) : typctx' :=
+  mkΔ (\{A} \u Δvars Δ) (Δeqs Δ).
+Definition add_eq' (Δ : typctx') (eq : type_equation) : typctx' :=
+  mkΔ (Δvars Δ) (\{eq} \u Δeqs Δ).
+Definition emptyΔ' := mkΔ \{} \{}.
 
-Fixpoint translate (Δ' : typctx') : typctx :=
-  match Δ' with
-  | [] => emptyΔ
-  | (tc_var A) :: Δ'' => add_var (translate Δ'') A
-  | (tc_eq eq) :: Δ'' => add_eq  (translate Δ'') eq
+Fixpoint translate (Δ : typctx) : typctx' :=
+  match Δ with
+  | [] => emptyΔ'
+  | (tc_var A) :: Δt => add_var' (translate Δt) A
+  | (tc_eq eq) :: Δt => add_eq'  (translate Δt) eq
   end.
 
-Inductive subst_matches_typctx' Σ : typctx' -> substitution -> Prop :=
-| tc_empty : subst_matches_typctx' Σ [] []
-| tc_add_var : forall Θ Δ A T,
-    wft Σ (translate Δ) T ->
-    subst_matches_typctx' Σ Δ Θ ->
-    subst_matches_typctx' Σ (tc_var A :: Δ) ((A, T) :: Θ)
-| tc_add_eq : forall Θ Δ T1 T2,
-    subst_matches_typctx' Σ Δ Θ ->
-    alpha_equivalent (subst_tt' T1 Θ) (subst_tt' T2 Θ) ->
-    subst_matches_typctx' Σ (tc_eq (T1 ≡ T2) :: Δ) Θ.
+Definition subst_matches_typctx' Σ Δ Θ :=
+  substitution_sources Θ = Δvars Δ /\
+  (forall A T, In (A,T) Θ -> wft Σ emptyΔ T) /\
+  (forall T1 T2, (T1 ≡ T2) \in (Δeqs Δ) ->
+            alpha_equivalent (subst_tt' T1 Θ) (subst_tt' T2 Θ)).
 
-(* TODO move this to proper place *)
-Lemma wft_strengthen_var : forall T Σ Δ A,
-    wft Σ Δ T ->
-    wft Σ (add_var Δ A) T.
-  induction 1; econstructor; eauto.
-  - destruct Δ as [vars ?].
-    cbn in *. auto.
-  - apply H0.
+(* Lemma wft_strengthen_var : forall T Σ Δ A, *)
+(*     wft Σ Δ T -> *)
+(*     wft Σ (add_var Δ A) T. *)
+(*   induction 1; econstructor; eauto. *)
+(*   - destruct Δ as [vars ?]. *)
+(*     cbn in *. *)
+(*     rewrite in_union. right*. *)
+(*   - intros. *)
+(*     assert (Hcom: add_var (add_var Δ A) X = add_var (add_var Δ X) A). *)
+(*     + cbv. f_equal. *)
+(*       rewrite union_assoc. *)
+(*       rewrite (union_comm \{X} \{A}). *)
+(*       rewrite <- union_assoc. *)
+(*       trivial. *)
+(*     + rewrite Hcom. apply H0. eauto. *)
+(* Qed. *)
+
+(* Lemma subst_extend: *)
+(*   forall (Θ : list (var * typ)) A (T T1 T2 : typ), *)
+(*     subst_tt' T1 Θ = subst_tt' T2 Θ -> *)
+(*     subst_tt' (subst_tt A T T1) Θ = subst_tt' (subst_tt A T T2) Θ. *)
+(* Proof. *)
+(*   induction Θ as [| (X, U) Θ]; introv IHC. *)
+(*   - cbn in *. subst. trivial. *)
+(*   - cbn. cbn in IHC. *)
+(*     apply IHΘ. *)
+(*     rewrite  subst_hmm. *)
+
+(* Lemma subst_reverse : forall Θ T1 T2 A U, *)
+(*   subst_tt A U (subst_tt' T1 Θ) = subst_tt A U (subst_tt' T2 Θ) -> *)
+(*   subst_tt' (subst_tt A U T1) Θ = subst_tt' (subst_tt A U T2) Θ. *)
+(*   induction Θ as [| (X, V) Θ]; introv IHC. *)
+(*   - cbn in *. auto. *)
+(*   - cbn in *. *)
+(*     lets HA: subst_hmm T1 T2 X A V. *)
+(*     lets HB: HA U. *)
+(*     lets IH: IHΘ (subst_tt A U T1) (subst_tt A U T2) X V. *)
+(*     apply IH. *)
+(*     f_equal. *)
+(*     apply IHΘ. *)
+(* Abort. *)
+
+Definition entails_semantic' Σ (Δ' : typctx') (eq : type_equation) :=
+  match eq with
+  | T1 ≡ T2 =>
+    forall Θ, subst_matches_typctx' Σ Δ' Θ ->
+         alpha_equivalent (subst_tt' T1 Θ) (subst_tt' T2 Θ)
+  end.
+
+Lemma empty_concat_inv : forall A (x : A) B,
+    \{} = \{x} \u B -> False.
+  intros.
+  assert (Hf: x \in \{}).
+  -- rewrite H.
+     rewrite in_union. left. rewrite in_singleton. trivial.
+  -- rewrite in_empty in Hf. trivial.
+Qed.
+
+(* Theorem subst_equivalence : forall Δ' Σ Δ, *)
+(*     okGadt Σ -> *)
+(*     translate Δ' = Δ -> *)
+(*     forall Θ, *)
+(*     subst_matches_typctx' Σ Δ' Θ <-> subst_matches_typctx Σ Δ Θ *)
+(*     . *)
+(*   induction Δ'; introv HokΣ Htranslate. *)
+(*   - cbn in Htranslate. subst. *)
+(*     intuition. *)
+(*     + inversions H. *)
+(*       unfold subst_matches_typctx. *)
+(*       splits*. *)
+(*       * intros; contradiction. *)
+(*       * intros. *)
+(*         cbv in H. rewrite in_empty in H. contradiction. *)
+(*     + destruct H as [? [? ?]]. *)
+(*       cbn in *. *)
+(*       destruct Θ. *)
+(*       * econstructor. *)
+(*       * exfalso. *)
+(*         cbn in H. *)
+(*         apply* empty_concat_inv. *)
+(*   - destruct a; cbn in Htranslate. *)
+(*     + constructor; introv Hsm; subst. *)
+(*       * admit. *)
+(*       * destruct Hsm as [Hsrc [Hwft Haeq]]. *)
+(*         destruct Θ as [| (X,V) Θ']. *)
+(*         -- cbn in Hsrc. *)
+(*            exfalso; apply* empty_concat_inv. *)
+(*         -- assert (X = A). *)
+(*            ++ admit. *)
+(*            ++ subst. apply tc_add_var. *)
+(*               ** apply wft_strengthen_var. *)
 
 
-Lemma wft_strengthen_var : forall T Σ Δ A,
-    wft Σ Δ T ->
-    wft Σ (add_var Δ A) T.
+(*       * constructor; intro H. *)
+(*         -- inversion H. *)
+(*         -- inversion H as [? [? ?]]. *)
+(*            destruct Δ as [vars ?]. *)
+(*            cbn in *. *)
+(*            subst. *)
+(*            inversion Htranslate. *)
+(*            assert (Hf: A \in \{}). *)
+(*            ++ rewrite <- H3. *)
+(*               rewrite in_union. left. rewrite in_singleton. trivial. *)
+(*            ++ rewrite in_empty in Hf; contradiction. *)
+    (*   * lets* [IH1 IH2]: IHΔ' Θ' Σ (translate Δ'). *)
+    (*     intuition. *)
+    (*     -- inversions H. *)
+    (*        lets [IHA [IHB IHC]]: IH1 H6. *)
+    (*        unfold subst_matches_typctx. *)
+    (*        splits*. *)
+    (*        ++ cbn. rewrite <- IHA. auto. *)
+    (*        ++ introv Hin. *)
+    (*           destruct Hin. *)
+    (*           ** inversions H. *)
+    (*              apply* wft_strengthen_var. *)
+    (*           ** apply* wft_strengthen_var. *)
+    (*        ++ introv Hin. *)
+    (*           unfold alpha_equivalent in *. *)
+    (*           cbn in Hin. *)
+    (*           cbn. *)
+    (*           admit. *)
+    (*     -- admit. *)
+    (* + constructor; intro H. *)
+    (*   * admit. *)
+    (*   * admit. *)
 
-Theorem equivalence : forall Δ' Θ Σ Δ,
-    okGadt Σ ->
-    translate Δ' = Δ ->
-    subst_matches_typctx' Σ Δ' Θ <-> subst_matches_typctx Σ Δ Θ
-    .
-  induction Δ'; introv HokΣ Htranslate.
-  - cbn in Htranslate. subst.
-    intuition.
-    + inversions H.
-      unfold subst_matches_typctx.
-      splits*.
-      * intros; contradiction.
-      * intros; contradiction.
-    + destruct H as [? [? ?]].
-      cbn in *.
-      destruct Θ.
-      * econstructor.
-      * exfalso.
-        cbn in H.
-        congruence.
-  - destruct a. cbn in Htranslate.
-    + destruct Θ as [| (A',T') Θ'].
-      * intuition.
-        -- inversion H.
-        -- inversion H as [? [? ?]].
-           destruct Δ as [vars ?].
-           cbn in *.
-           subst.
-           inversion Htranslate.
-      * lets* [IH1 IH2]: IHΔ' Θ' Σ (translate Δ').
-        intuition.
-        -- inversions H.
-           lets [IHA [IHB IHC]]: IH1 H6.
-           unfold subst_matches_typctx.
-           splits*.
-           ++ cbn. rewrite <- IHA. auto.
-           ++ 
-    + 
-    Admitted.
-
-
+Theorem equivalence : forall Δ' Δ,
+    translate Δ = Δ' ->
+    forall Σ T1 T2,
+      okGadt Σ ->
+      entails_semantic' Σ Δ' (T1 ≡ T2) <-> entails_semantic Σ Δ (T1 ≡ T2).
+  introv Htr. induction T1; destruct T2; introv Hgadt.
+  constructor; intro Hsem.
+  - unfold entails_semantic' in *; unfold entails_semantic in *;
+      unfold alpha_equivalent in *.
+    introv HΘ.
+  (* introv Htr Hgadt. *)
+  (* constructor; introv Hentails; *)
+  (*   unfold entails_semantic' in *; unfold entails_semantic in *; *)
+  (*     introv Hmatch; *)
+  (*     apply Hentails; *)
+  (*     lets Heq: subst_equivalence Hgadt Htr; *)
+  (*     apply* Heq. *)
+Abort.
 
 End TypCtxDefEquivalence.
